pulse/src/ocaml/plugin/generated/Pulse_Checker_While.ml
@@ -2,31 +2,35 @@ open Prims
 let (while_cond_comp_typing :
   Pulse_Typing_Env.env ->
     Pulse_Syntax_Base.universe ->
-      Pulse_Syntax_Base.term ->
+      Pulse_Syntax_Base.ppname ->
         Pulse_Syntax_Base.term ->
-          unit -> (unit, unit) Pulse_Typing_Metatheory.comp_typing_u)
+          Pulse_Syntax_Base.term ->
+            unit -> (unit, unit) Pulse_Typing_Metatheory.comp_typing_u)
   =
   fun g ->
     fun u ->
-      fun ty ->
-        fun inv_body ->
-          fun inv_typing ->
-            Pulse_Typing_Metatheory.admit_comp_typing g
-              (Pulse_Typing.comp_while_cond inv_body)
+      fun x ->
+        fun ty ->
+          fun inv_body ->
+            fun inv_typing ->
+              Pulse_Typing_Metatheory.admit_comp_typing g
+                (Pulse_Typing.comp_while_cond x inv_body)
 let (while_body_comp_typing :
   Pulse_Typing_Env.env ->
     Pulse_Syntax_Base.universe ->
-      Pulse_Syntax_Base.term ->
+      Pulse_Syntax_Base.ppname ->
         Pulse_Syntax_Base.term ->
-          unit -> (unit, unit) Pulse_Typing_Metatheory.comp_typing_u)
+          Pulse_Syntax_Base.term ->
+            unit -> (unit, unit) Pulse_Typing_Metatheory.comp_typing_u)
   =
   fun g ->
     fun u ->
-      fun ty ->
-        fun inv_body ->
-          fun inv_typing ->
-            Pulse_Typing_Metatheory.admit_comp_typing g
-              (Pulse_Typing.comp_while_body inv_body)
+      fun x ->
+        fun ty ->
+          fun inv_body ->
+            fun inv_typing ->
+              Pulse_Typing_Metatheory.admit_comp_typing g
+                (Pulse_Typing.comp_while_body x inv_body)
 let (check_while :
   Prims.bool ->
     Pulse_Typing_Env.env ->
@@ -51,7 +55,7 @@ let (check_while :
                      (Prims.of_int (37)) (Prims.of_int (37)))
                   (FStar_Range.mk_range "Pulse.Checker.While.fst"
                      (Prims.of_int (37)) (Prims.of_int (40))
-                     (Prims.of_int (114)) (Prims.of_int (59)))
+                     (Prims.of_int (108)) (Prims.of_int (59)))
                   (FStar_Tactics_Effect.lift_div_tac
                      (fun uu___ ->
                         Pulse_Checker_Pure.push_context "while loop" g))
@@ -64,7 +68,7 @@ let (check_while :
                                 (Prims.of_int (38)) (Prims.of_int (78)))
                              (FStar_Range.mk_range "Pulse.Checker.While.fst"
                                 (Prims.of_int (37)) (Prims.of_int (40))
-                                (Prims.of_int (114)) (Prims.of_int (59)))
+                                (Prims.of_int (108)) (Prims.of_int (59)))
                              (FStar_Tactics_Effect.lift_div_tac
                                 (fun uu___ -> t.Pulse_Syntax_Base.term1))
                              (fun uu___ ->
@@ -81,130 +85,29 @@ let (check_while :
                                          (FStar_Tactics_Effect.tac_bind
                                             (FStar_Range.mk_range
                                                "Pulse.Checker.While.fst"
-                                               (Prims.of_int (39))
-                                               (Prims.of_int (32))
-                                               (Prims.of_int (46))
-                                               (Prims.of_int (48)))
+                                               (Prims.of_int (40))
+                                               (Prims.of_int (4))
+                                               (Prims.of_int (40))
+                                               (Prims.of_int (116)))
                                             (FStar_Range.mk_range
                                                "Pulse.Checker.While.fst"
                                                (Prims.of_int (38))
                                                (Prims.of_int (81))
-                                               (Prims.of_int (114))
+                                               (Prims.of_int (108))
                                                (Prims.of_int (59)))
                                             (Obj.magic
-                                               (FStar_Tactics_Effect.tac_bind
-                                                  (FStar_Range.mk_range
-                                                     "Pulse.Checker.While.fst"
-                                                     (Prims.of_int (40))
-                                                     (Prims.of_int (30))
-                                                     (Prims.of_int (40))
-                                                     (Prims.of_int (101)))
-                                                  (FStar_Range.mk_range
-                                                     "Pulse.Checker.While.fst"
-                                                     (Prims.of_int (42))
-                                                     (Prims.of_int (4))
-                                                     (Prims.of_int (46))
-                                                     (Prims.of_int (48)))
-                                                  (FStar_Tactics_Effect.lift_div_tac
-                                                     (fun uu___1 ->
-                                                        Pulse_Syntax_Base.Tm_ExistsSL
-                                                          (Pulse_Syntax_Pure.u0,
-                                                            {
-                                                              Pulse_Syntax_Base.binder_ty
-                                                                =
-                                                                Pulse_Typing.tm_bool;
-                                                              Pulse_Syntax_Base.binder_ppname
-                                                                =
-                                                                condition_var
-                                                            }, inv)))
-                                                  (fun uu___1 ->
-                                                     (fun inv1 ->
-                                                        Obj.magic
-                                                          (FStar_Tactics_Effect.tac_bind
-                                                             (FStar_Range.mk_range
-                                                                "Pulse.Checker.While.fst"
-                                                                (Prims.of_int (42))
-                                                                (Prims.of_int (4))
-                                                                (Prims.of_int (45))
-                                                                (Prims.of_int (5)))
-                                                             (FStar_Range.mk_range
-                                                                "Pulse.Checker.While.fst"
-                                                                (Prims.of_int (46))
-                                                                (Prims.of_int (4))
-                                                                (Prims.of_int (46))
-                                                                (Prims.of_int (48)))
-                                                             (if
-                                                                Pulse_RuntimeUtils.debug_at_level
-                                                                  g1
-                                                                  "inference"
-                                                              then
-                                                                Obj.magic
-                                                                  (Obj.repr
-                                                                    (FStar_Tactics_Effect.tac_bind
-                                                                    (FStar_Range.mk_range
-                                                                    "Pulse.Checker.While.fst"
-                                                                    (Prims.of_int (44))
-                                                                    (Prims.of_int (14))
-                                                                    (Prims.of_int (44))
-                                                                    (Prims.of_int (98)))
-                                                                    (FStar_Range.mk_range
-                                                                    "Pulse.Checker.While.fst"
-                                                                    (Prims.of_int (43))
-                                                                    (Prims.of_int (9))
-                                                                    (Prims.of_int (45))
-                                                                    (Prims.of_int (5)))
-                                                                    (Obj.magic
-                                                                    (FStar_Tactics_Effect.tac_bind
-                                                                    (FStar_Range.mk_range
-                                                                    "Pulse.Checker.While.fst"
-                                                                    (Prims.of_int (44))
-                                                                    (Prims.of_int (75))
-                                                                    (Prims.of_int (44))
-                                                                    (Prims.of_int (97)))
-                                                                    (FStar_Range.mk_range
-                                                                    "prims.fst"
-                                                                    (Prims.of_int (590))
-                                                                    (Prims.of_int (19))
-                                                                    (Prims.of_int (590))
-                                                                    (Prims.of_int (31)))
-                                                                    (Obj.magic
-                                                                    (Pulse_Syntax_Printer.term_to_string
-                                                                    inv1))
-                                                                    (fun
-                                                                    uu___1 ->
-                                                                    FStar_Tactics_Effect.lift_div_tac
-                                                                    (fun
-                                                                    uu___2 ->
-                                                                    Prims.strcat
-                                                                    "Annotated precondition of while loop: "
-                                                                    (Prims.strcat
-                                                                    uu___1
-                                                                    "\n")))))
-                                                                    (fun
-                                                                    uu___1 ->
-                                                                    (fun
-                                                                    uu___1 ->
-                                                                    Obj.magic
-                                                                    (FStar_Tactics_Builtins.print
-                                                                    uu___1))
-                                                                    uu___1)))
-                                                              else
-                                                                Obj.magic
-                                                                  (Obj.repr
-                                                                    (FStar_Tactics_Effect.lift_div_tac
-                                                                    (fun
-                                                                    uu___2 ->
-                                                                    ()))))
-                                                             (fun uu___1 ->
-                                                                (fun uu___1
-                                                                   ->
-                                                                   Obj.magic
-                                                                    (Pulse_Checker_Pure.check_vprop
-                                                                    (Pulse_Checker_Pure.push_context
-                                                                    "invariant"
-                                                                    g1) inv1))
-                                                                  uu___1)))
-                                                       uu___1)))
+                                               (Pulse_Checker_Pure.check_vprop
+                                                  (Pulse_Checker_Pure.push_context
+                                                     "invariant" g1)
+                                                  (Pulse_Syntax_Base.Tm_ExistsSL
+                                                     (Pulse_Syntax_Pure.u0,
+                                                       {
+                                                         Pulse_Syntax_Base.binder_ty
+                                                           =
+                                                           Pulse_Typing.tm_bool;
+                                                         Pulse_Syntax_Base.binder_ppname
+                                                           = condition_var
+                                                       }, inv))))
                                             (fun uu___1 ->
                                                (fun uu___1 ->
                                                   match uu___1 with
@@ -214,15 +117,15 @@ let (check_while :
                                                         (FStar_Tactics_Effect.tac_bind
                                                            (FStar_Range.mk_range
                                                               "Pulse.Checker.While.fst"
-                                                              (Prims.of_int (48))
+                                                              (Prims.of_int (42))
                                                               (Prims.of_int (2))
-                                                              (Prims.of_int (51))
+                                                              (Prims.of_int (45))
                                                               (Prims.of_int (3)))
                                                            (FStar_Range.mk_range
                                                               "Pulse.Checker.While.fst"
-                                                              (Prims.of_int (52))
+                                                              (Prims.of_int (46))
                                                               (Prims.of_int (2))
-                                                              (Prims.of_int (114))
+                                                              (Prims.of_int (108))
                                                               (Prims.of_int (59)))
                                                            (if
                                                               Pulse_RuntimeUtils.debug_at_level
@@ -234,23 +137,23 @@ let (check_while :
                                                                    (FStar_Tactics_Effect.tac_bind
                                                                     (FStar_Range.mk_range
                                                                     "Pulse.Checker.While.fst"
-                                                                    (Prims.of_int (50))
+                                                                    (Prims.of_int (44))
                                                                     (Prims.of_int (12))
-                                                                    (Prims.of_int (50))
+                                                                    (Prims.of_int (44))
                                                                     (Prims.of_int (98)))
                                                                     (FStar_Range.mk_range
                                                                     "Pulse.Checker.While.fst"
-                                                                    (Prims.of_int (49))
+                                                                    (Prims.of_int (43))
                                                                     (Prims.of_int (7))
-                                                                    (Prims.of_int (51))
+                                                                    (Prims.of_int (45))
                                                                     (Prims.of_int (3)))
                                                                     (Obj.magic
                                                                     (FStar_Tactics_Effect.tac_bind
                                                                     (FStar_Range.mk_range
                                                                     "Pulse.Checker.While.fst"
-                                                                    (Prims.of_int (50))
+                                                                    (Prims.of_int (44))
                                                                     (Prims.of_int (72))
-                                                                    (Prims.of_int (50))
+                                                                    (Prims.of_int (44))
                                                                     (Prims.of_int (97)))
                                                                     (FStar_Range.mk_range
                                                                     "prims.fst"
@@ -292,15 +195,15 @@ let (check_while :
                                                                    (FStar_Tactics_Effect.tac_bind
                                                                     (FStar_Range.mk_range
                                                                     "Pulse.Checker.While.fst"
-                                                                    (Prims.of_int (52))
+                                                                    (Prims.of_int (46))
                                                                     (Prims.of_int (8))
-                                                                    (Prims.of_int (52))
+                                                                    (Prims.of_int (46))
                                                                     (Prims.of_int (49)))
                                                                     (FStar_Range.mk_range
                                                                     "Pulse.Checker.While.fst"
-                                                                    (Prims.of_int (52))
+                                                                    (Prims.of_int (46))
                                                                     (Prims.of_int (2))
-                                                                    (Prims.of_int (114))
+                                                                    (Prims.of_int (108))
                                                                     (Prims.of_int (59)))
                                                                     (Obj.magic
                                                                     (Pulse_Checker_Framing.check_frameable
@@ -335,7 +238,7 @@ let (check_while :
                                                                     Pulse_Syntax_Base.binder_ty
                                                                     = ty;
                                                                     Pulse_Syntax_Base.binder_ppname
-                                                                    = uu___4;_},
+                                                                    = nm;_},
                                                                     inv1) ->
                                                                     Obj.repr
                                                                     (if
@@ -357,26 +260,27 @@ let (check_while :
                                                                     (FStar_Tactics_Effect.tac_bind
                                                                     (FStar_Range.mk_range
                                                                     "Pulse.Checker.While.fst"
-                                                                    (Prims.of_int (61))
+                                                                    (Prims.of_int (55))
                                                                     (Prims.of_int (37))
-                                                                    (Prims.of_int (61))
-                                                                    (Prims.of_int (79)))
+                                                                    (Prims.of_int (55))
+                                                                    (Prims.of_int (82)))
                                                                     (FStar_Range.mk_range
                                                                     "Pulse.Checker.While.fst"
-                                                                    (Prims.of_int (61))
-                                                                    (Prims.of_int (82))
-                                                                    (Prims.of_int (112))
-                                                                    (Prims.of_int (74)))
+                                                                    (Prims.of_int (55))
+                                                                    (Prims.of_int (85))
+                                                                    (Prims.of_int (106))
+                                                                    (Prims.of_int (77)))
                                                                     (FStar_Tactics_Effect.lift_div_tac
                                                                     (fun
-                                                                    uu___6 ->
+                                                                    uu___5 ->
                                                                     while_cond_comp_typing
                                                                     (Pulse_Checker_Pure.push_context
                                                                     "invariant"
-                                                                    g1) u ty
-                                                                    inv1 ()))
+                                                                    g1) u nm
+                                                                    ty inv1
+                                                                    ()))
                                                                     (fun
-                                                                    uu___6 ->
+                                                                    uu___5 ->
                                                                     (fun
                                                                     while_cond_comp_typing1
                                                                     ->
@@ -384,38 +288,38 @@ let (check_while :
                                                                     (FStar_Tactics_Effect.tac_bind
                                                                     (FStar_Range.mk_range
                                                                     "Pulse.Checker.While.fst"
-                                                                    (Prims.of_int (63))
+                                                                    (Prims.of_int (57))
                                                                     (Prims.of_int (24))
-                                                                    (Prims.of_int (63))
+                                                                    (Prims.of_int (57))
                                                                     (Prims.of_int (95)))
                                                                     (FStar_Range.mk_range
                                                                     "Pulse.Checker.While.fst"
-                                                                    (Prims.of_int (61))
-                                                                    (Prims.of_int (82))
-                                                                    (Prims.of_int (112))
-                                                                    (Prims.of_int (74)))
+                                                                    (Prims.of_int (55))
+                                                                    (Prims.of_int (85))
+                                                                    (Prims.of_int (106))
+                                                                    (Prims.of_int (77)))
                                                                     (FStar_Tactics_Effect.lift_div_tac
                                                                     (fun
-                                                                    uu___6 ->
+                                                                    uu___5 ->
                                                                     Pulse_Typing_Metatheory.st_comp_typing_inversion
                                                                     (Pulse_Checker_Pure.push_context
                                                                     "invariant"
                                                                     g1)
                                                                     (Pulse_Syntax_Base.st_comp_of_comp
                                                                     (Pulse_Typing.comp_while_cond
-                                                                    inv1))
+                                                                    nm inv1))
                                                                     (Pulse_Typing_Metatheory.comp_typing_inversion
                                                                     (Pulse_Checker_Pure.push_context
                                                                     "invariant"
                                                                     g1)
                                                                     (Pulse_Typing.comp_while_cond
-                                                                    inv1)
+                                                                    nm inv1)
                                                                     while_cond_comp_typing1)))
                                                                     (fun
-                                                                    uu___6 ->
+                                                                    uu___5 ->
                                                                     (fun
-                                                                    uu___6 ->
-                                                                    match uu___6
+                                                                    uu___5 ->
+                                                                    match uu___5
                                                                     with
                                                                     | 
                                                                     FStar_Pervasives.Mkdtuple4
@@ -428,28 +332,28 @@ let (check_while :
                                                                     (FStar_Tactics_Effect.tac_bind
                                                                     (FStar_Range.mk_range
                                                                     "Pulse.Checker.While.fst"
-                                                                    (Prims.of_int (67))
+                                                                    (Prims.of_int (61))
                                                                     (Prims.of_int (12))
-                                                                    (Prims.of_int (67))
+                                                                    (Prims.of_int (61))
                                                                     (Prims.of_int (61)))
                                                                     (FStar_Range.mk_range
                                                                     "Pulse.Checker.While.fst"
-                                                                    (Prims.of_int (68))
+                                                                    (Prims.of_int (62))
                                                                     (Prims.of_int (10))
-                                                                    (Prims.of_int (112))
-                                                                    (Prims.of_int (74)))
+                                                                    (Prims.of_int (106))
+                                                                    (Prims.of_int (77)))
                                                                     (FStar_Tactics_Effect.lift_div_tac
                                                                     (fun
-                                                                    uu___7 ->
+                                                                    uu___6 ->
                                                                     Pulse_Checker_Common.post_hint_from_comp_typing
                                                                     (Pulse_Checker_Pure.push_context
                                                                     "invariant"
                                                                     g1)
                                                                     (Pulse_Typing.comp_while_cond
-                                                                    inv1)
+                                                                    nm inv1)
                                                                     while_cond_comp_typing1))
                                                                     (fun
-                                                                    uu___7 ->
+                                                                    uu___6 ->
                                                                     (fun
                                                                     while_cond_hint
                                                                     ->
@@ -457,16 +361,16 @@ let (check_while :
                                                                     (FStar_Tactics_Effect.tac_bind
                                                                     (FStar_Range.mk_range
                                                                     "Pulse.Checker.While.fst"
-                                                                    (Prims.of_int (70))
+                                                                    (Prims.of_int (64))
                                                                     (Prims.of_int (10))
-                                                                    (Prims.of_int (75))
+                                                                    (Prims.of_int (69))
                                                                     (Prims.of_int (39)))
                                                                     (FStar_Range.mk_range
                                                                     "Pulse.Checker.While.fst"
-                                                                    (Prims.of_int (68))
+                                                                    (Prims.of_int (62))
                                                                     (Prims.of_int (10))
-                                                                    (Prims.of_int (112))
-                                                                    (Prims.of_int (74)))
+                                                                    (Prims.of_int (106))
+                                                                    (Prims.of_int (77)))
                                                                     (Obj.magic
                                                                     (check'
                                                                     allow_inst
@@ -475,14 +379,15 @@ let (check_while :
                                                                     g1) cond
                                                                     (Pulse_Syntax_Base.comp_pre
                                                                     (Pulse_Typing.comp_while_cond
-                                                                    inv1)) ()
+                                                                    nm inv1))
+                                                                    ()
                                                                     (FStar_Pervasives_Native.Some
                                                                     while_cond_hint)))
                                                                     (fun
-                                                                    uu___7 ->
+                                                                    uu___6 ->
                                                                     (fun
-                                                                    uu___7 ->
-                                                                    match uu___7
+                                                                    uu___6 ->
+                                                                    match uu___6
                                                                     with
                                                                     | 
                                                                     FStar_Pervasives.Mkdtuple3
@@ -494,32 +399,33 @@ let (check_while :
                                                                     Pulse_Syntax_Base.eq_comp
                                                                     cond_comp
                                                                     (Pulse_Typing.comp_while_cond
-                                                                    inv1)
+                                                                    nm inv1)
                                                                     then
                                                                     Obj.magic
                                                                     (FStar_Tactics_Effect.tac_bind
                                                                     (FStar_Range.mk_range
                                                                     "Pulse.Checker.While.fst"
-                                                                    (Prims.of_int (79))
+                                                                    (Prims.of_int (73))
                                                                     (Prims.of_int (39))
-                                                                    (Prims.of_int (79))
-                                                                    (Prims.of_int (81)))
+                                                                    (Prims.of_int (73))
+                                                                    (Prims.of_int (84)))
                                                                     (FStar_Range.mk_range
                                                                     "Pulse.Checker.While.fst"
-                                                                    (Prims.of_int (79))
-                                                                    (Prims.of_int (84))
-                                                                    (Prims.of_int (105))
-                                                                    (Prims.of_int (78)))
+                                                                    (Prims.of_int (73))
+                                                                    (Prims.of_int (87))
+                                                                    (Prims.of_int (99))
+                                                                    (Prims.of_int (81)))
                                                                     (FStar_Tactics_Effect.lift_div_tac
                                                                     (fun
-                                                                    uu___8 ->
+                                                                    uu___7 ->
                                                                     while_body_comp_typing
                                                                     (Pulse_Checker_Pure.push_context
                                                                     "invariant"
-                                                                    g1) u ty
-                                                                    inv1 ()))
+                                                                    g1) u nm
+                                                                    ty inv1
+                                                                    ()))
                                                                     (fun
-                                                                    uu___8 ->
+                                                                    uu___7 ->
                                                                     (fun
                                                                     while_body_comp_typing1
                                                                     ->
@@ -527,38 +433,38 @@ let (check_while :
                                                                     (FStar_Tactics_Effect.tac_bind
                                                                     (FStar_Range.mk_range
                                                                     "Pulse.Checker.While.fst"
-                                                                    (Prims.of_int (81))
+                                                                    (Prims.of_int (75))
                                                                     (Prims.of_int (26))
-                                                                    (Prims.of_int (81))
+                                                                    (Prims.of_int (75))
                                                                     (Prims.of_int (97)))
                                                                     (FStar_Range.mk_range
                                                                     "Pulse.Checker.While.fst"
-                                                                    (Prims.of_int (79))
-                                                                    (Prims.of_int (84))
-                                                                    (Prims.of_int (105))
-                                                                    (Prims.of_int (78)))
+                                                                    (Prims.of_int (73))
+                                                                    (Prims.of_int (87))
+                                                                    (Prims.of_int (99))
+                                                                    (Prims.of_int (81)))
                                                                     (FStar_Tactics_Effect.lift_div_tac
                                                                     (fun
-                                                                    uu___8 ->
+                                                                    uu___7 ->
                                                                     Pulse_Typing_Metatheory.st_comp_typing_inversion
                                                                     (Pulse_Checker_Pure.push_context
                                                                     "invariant"
                                                                     g1)
                                                                     (Pulse_Syntax_Base.st_comp_of_comp
                                                                     (Pulse_Typing.comp_while_body
-                                                                    inv1))
+                                                                    nm inv1))
                                                                     (Pulse_Typing_Metatheory.comp_typing_inversion
                                                                     (Pulse_Checker_Pure.push_context
                                                                     "invariant"
                                                                     g1)
                                                                     (Pulse_Typing.comp_while_body
-                                                                    inv1)
+                                                                    nm inv1)
                                                                     while_body_comp_typing1)))
                                                                     (fun
-                                                                    uu___8 ->
+                                                                    uu___7 ->
                                                                     (fun
-                                                                    uu___8 ->
-                                                                    match uu___8
+                                                                    uu___7 ->
+                                                                    match uu___7
                                                                     with
                                                                     | 
                                                                     FStar_Pervasives.Mkdtuple4
@@ -571,28 +477,28 @@ let (check_while :
                                                                     (FStar_Tactics_Effect.tac_bind
                                                                     (FStar_Range.mk_range
                                                                     "Pulse.Checker.While.fst"
-                                                                    (Prims.of_int (85))
+                                                                    (Prims.of_int (79))
                                                                     (Prims.of_int (14))
-                                                                    (Prims.of_int (85))
+                                                                    (Prims.of_int (79))
                                                                     (Prims.of_int (63)))
                                                                     (FStar_Range.mk_range
                                                                     "Pulse.Checker.While.fst"
-                                                                    (Prims.of_int (86))
+                                                                    (Prims.of_int (80))
                                                                     (Prims.of_int (12))
-                                                                    (Prims.of_int (105))
-                                                                    (Prims.of_int (78)))
+                                                                    (Prims.of_int (99))
+                                                                    (Prims.of_int (81)))
                                                                     (FStar_Tactics_Effect.lift_div_tac
                                                                     (fun
-                                                                    uu___9 ->
+                                                                    uu___8 ->
                                                                     Pulse_Checker_Common.post_hint_from_comp_typing
                                                                     (Pulse_Checker_Pure.push_context
                                                                     "invariant"
                                                                     g1)
                                                                     (Pulse_Typing.comp_while_body
-                                                                    inv1)
+                                                                    nm inv1)
                                                                     while_body_comp_typing1))
                                                                     (fun
-                                                                    uu___9 ->
+                                                                    uu___8 ->
                                                                     (fun
                                                                     while_post_hint
                                                                     ->
@@ -600,16 +506,16 @@ let (check_while :
                                                                     (FStar_Tactics_Effect.tac_bind
                                                                     (FStar_Range.mk_range
                                                                     "Pulse.Checker.While.fst"
-                                                                    (Prims.of_int (88))
+                                                                    (Prims.of_int (82))
                                                                     (Prims.of_int (14))
-                                                                    (Prims.of_int (93))
+                                                                    (Prims.of_int (87))
                                                                     (Prims.of_int (43)))
                                                                     (FStar_Range.mk_range
                                                                     "Pulse.Checker.While.fst"
-                                                                    (Prims.of_int (86))
+                                                                    (Prims.of_int (80))
                                                                     (Prims.of_int (12))
-                                                                    (Prims.of_int (105))
-                                                                    (Prims.of_int (78)))
+                                                                    (Prims.of_int (99))
+                                                                    (Prims.of_int (81)))
                                                                     (Obj.magic
                                                                     (check'
                                                                     allow_inst
@@ -618,14 +524,15 @@ let (check_while :
                                                                     g1) body
                                                                     (Pulse_Syntax_Base.comp_pre
                                                                     (Pulse_Typing.comp_while_body
-                                                                    inv1)) ()
+                                                                    nm inv1))
+                                                                    ()
                                                                     (FStar_Pervasives_Native.Some
                                                                     while_post_hint)))
                                                                     (fun
-                                                                    uu___9 ->
+                                                                    uu___8 ->
                                                                     (fun
-                                                                    uu___9 ->
-                                                                    match uu___9
+                                                                    uu___8 ->
+                                                                    match uu___8
                                                                     with
                                                                     | 
                                                                     FStar_Pervasives.Mkdtuple3
@@ -637,26 +544,25 @@ let (check_while :
                                                                     Pulse_Syntax_Base.eq_comp
                                                                     body_comp
                                                                     (Pulse_Typing.comp_while_body
-                                                                    inv1)
+                                                                    nm inv1)
                                                                     then
                                                                     Obj.magic
                                                                     (FStar_Tactics_Effect.tac_bind
                                                                     (FStar_Range.mk_range
                                                                     "Pulse.Checker.While.fst"
-                                                                    (Prims.of_int (96))
+                                                                    (Prims.of_int (90))
                                                                     (Prims.of_int (23))
-                                                                    (Prims.of_int (96))
+                                                                    (Prims.of_int (90))
                                                                     (Prims.of_int (81)))
                                                                     (FStar_Range.mk_range
                                                                     "Pulse.Checker.While.fst"
-                                                                    (Prims.of_int (96))
+                                                                    (Prims.of_int (90))
                                                                     (Prims.of_int (84))
-                                                                    (Prims.of_int (98))
+                                                                    (Prims.of_int (92))
                                                                     (Prims.of_int (45)))
                                                                     (FStar_Tactics_Effect.lift_div_tac
                                                                     (fun
-                                                                    uu___10
-                                                                    ->
+                                                                    uu___9 ->
                                                                     Pulse_Typing.T_While
                                                                     (g1,
                                                                     inv1,
@@ -666,27 +572,25 @@ let (check_while :
                                                                     cond_typing,
                                                                     body_typing)))
                                                                     (fun
-                                                                    uu___10
-                                                                    ->
+                                                                    uu___9 ->
                                                                     (fun d ->
                                                                     Obj.magic
                                                                     (FStar_Tactics_Effect.tac_bind
                                                                     (FStar_Range.mk_range
                                                                     "Pulse.Checker.While.fst"
-                                                                    (Prims.of_int (97))
+                                                                    (Prims.of_int (91))
                                                                     (Prims.of_int (35))
-                                                                    (Prims.of_int (97))
+                                                                    (Prims.of_int (91))
                                                                     (Prims.of_int (81)))
                                                                     (FStar_Range.mk_range
                                                                     "Pulse.Checker.While.fst"
-                                                                    (Prims.of_int (96))
+                                                                    (Prims.of_int (90))
                                                                     (Prims.of_int (84))
-                                                                    (Prims.of_int (98))
+                                                                    (Prims.of_int (92))
                                                                     (Prims.of_int (45)))
                                                                     (FStar_Tactics_Effect.lift_div_tac
                                                                     (fun
-                                                                    uu___10
-                                                                    ->
+                                                                    uu___9 ->
                                                                     Pulse_Checker_Framing.apply_frame
                                                                     g
                                                                     (Pulse_Typing.wr
@@ -704,15 +608,14 @@ let (check_while :
                                                                     })) pre
                                                                     ()
                                                                     (Pulse_Typing.comp_while
+                                                                    Pulse_Syntax_Base.ppname_default
                                                                     inv1) d
                                                                     framing_token))
                                                                     (fun
-                                                                    uu___10
-                                                                    ->
+                                                                    uu___9 ->
                                                                     (fun
-                                                                    uu___10
-                                                                    ->
-                                                                    match uu___10
+                                                                    uu___9 ->
+                                                                    match uu___9
                                                                     with
                                                                     | 
                                                                     Prims.Mkdtuple2
@@ -737,68 +640,68 @@ let (check_while :
                                                                     (Prims.Mkdtuple2
                                                                     (c, st_d))
                                                                     post_hint))
-                                                                    uu___10)))
-                                                                    uu___10))
+                                                                    uu___9)))
+                                                                    uu___9))
                                                                     else
                                                                     Obj.magic
                                                                     (FStar_Tactics_Effect.tac_bind
                                                                     (FStar_Range.mk_range
                                                                     "Pulse.Checker.While.fst"
-                                                                    (Prims.of_int (101))
+                                                                    (Prims.of_int (95))
                                                                     (Prims.of_int (14))
-                                                                    (Prims.of_int (105))
-                                                                    (Prims.of_int (78)))
+                                                                    (Prims.of_int (99))
+                                                                    (Prims.of_int (81)))
                                                                     (FStar_Range.mk_range
                                                                     "Pulse.Checker.While.fst"
-                                                                    (Prims.of_int (100))
+                                                                    (Prims.of_int (94))
                                                                     (Prims.of_int (12))
-                                                                    (Prims.of_int (105))
-                                                                    (Prims.of_int (78)))
+                                                                    (Prims.of_int (99))
+                                                                    (Prims.of_int (81)))
                                                                     (Obj.magic
                                                                     (FStar_Tactics_Effect.tac_bind
                                                                     (FStar_Range.mk_range
                                                                     "Pulse.Checker.While.fst"
-                                                                    (Prims.of_int (105))
+                                                                    (Prims.of_int (99))
                                                                     (Prims.of_int (37))
-                                                                    (Prims.of_int (105))
-                                                                    (Prims.of_int (77)))
+                                                                    (Prims.of_int (99))
+                                                                    (Prims.of_int (80)))
                                                                     (FStar_Range.mk_range
                                                                     "Pulse.Checker.While.fst"
-                                                                    (Prims.of_int (101))
+                                                                    (Prims.of_int (95))
                                                                     (Prims.of_int (14))
-                                                                    (Prims.of_int (105))
-                                                                    (Prims.of_int (78)))
+                                                                    (Prims.of_int (99))
+                                                                    (Prims.of_int (81)))
                                                                     (Obj.magic
                                                                     (Pulse_Syntax_Printer.comp_to_string
                                                                     (Pulse_Typing.comp_while_body
-                                                                    inv1)))
+                                                                    nm inv1)))
                                                                     (fun
-                                                                    uu___11
+                                                                    uu___10
                                                                     ->
                                                                     (fun
-                                                                    uu___11
+                                                                    uu___10
                                                                     ->
                                                                     Obj.magic
                                                                     (FStar_Tactics_Effect.tac_bind
                                                                     (FStar_Range.mk_range
                                                                     "Pulse.Checker.While.fst"
-                                                                    (Prims.of_int (101))
+                                                                    (Prims.of_int (95))
                                                                     (Prims.of_int (14))
-                                                                    (Prims.of_int (105))
-                                                                    (Prims.of_int (78)))
+                                                                    (Prims.of_int (99))
+                                                                    (Prims.of_int (81)))
                                                                     (FStar_Range.mk_range
                                                                     "Pulse.Checker.While.fst"
-                                                                    (Prims.of_int (101))
+                                                                    (Prims.of_int (95))
                                                                     (Prims.of_int (14))
-                                                                    (Prims.of_int (105))
-                                                                    (Prims.of_int (78)))
+                                                                    (Prims.of_int (99))
+                                                                    (Prims.of_int (81)))
                                                                     (Obj.magic
                                                                     (FStar_Tactics_Effect.tac_bind
                                                                     (FStar_Range.mk_range
                                                                     "Pulse.Checker.While.fst"
-                                                                    (Prims.of_int (104))
+                                                                    (Prims.of_int (98))
                                                                     (Prims.of_int (37))
-                                                                    (Prims.of_int (104))
+                                                                    (Prims.of_int (98))
                                                                     (Prims.of_int (65)))
                                                                     (FStar_Range.mk_range
                                                                     "FStar.Printf.fst"
@@ -810,98 +713,98 @@ let (check_while :
                                                                     (Pulse_Syntax_Printer.comp_to_string
                                                                     body_comp))
                                                                     (fun
-                                                                    uu___12
+                                                                    uu___11
                                                                     ->
                                                                     FStar_Tactics_Effect.lift_div_tac
                                                                     (fun
-                                                                    uu___13
+                                                                    uu___12
                                                                     ->
                                                                     fun x2 ->
                                                                     Prims.strcat
                                                                     (Prims.strcat
                                                                     "Could not prove the inferred type of the while body matches the annotation\nInferred type = "
                                                                     (Prims.strcat
-                                                                    uu___12
+                                                                    uu___11
                                                                     "\nAnnotated type = "))
                                                                     (Prims.strcat
                                                                     x2 "\n")))))
                                                                     (fun
-                                                                    uu___12
+                                                                    uu___11
                                                                     ->
                                                                     FStar_Tactics_Effect.lift_div_tac
                                                                     (fun
-                                                                    uu___13
-                                                                    ->
                                                                     uu___12
-                                                                    uu___11))))
-                                                                    uu___11)))
-                                                                    (fun
+                                                                    ->
                                                                     uu___11
+                                                                    uu___10))))
+                                                                    uu___10)))
+                                                                    (fun
+                                                                    uu___10
                                                                     ->
                                                                     FStar_Tactics_Derived.fail
-                                                                    uu___11)))
-                                                                    uu___9)))
-                                                                    uu___9)))
+                                                                    uu___10)))
                                                                     uu___8)))
-                                                                    uu___8))
+                                                                    uu___8)))
+                                                                    uu___7)))
+                                                                    uu___7))
                                                                     else
                                                                     Obj.magic
                                                                     (FStar_Tactics_Effect.tac_bind
                                                                     (FStar_Range.mk_range
                                                                     "Pulse.Checker.While.fst"
-                                                                    (Prims.of_int (108))
+                                                                    (Prims.of_int (102))
                                                                     Prims.int_zero
-                                                                    (Prims.of_int (112))
-                                                                    (Prims.of_int (74)))
+                                                                    (Prims.of_int (106))
+                                                                    (Prims.of_int (77)))
                                                                     (FStar_Range.mk_range
                                                                     "Pulse.Checker.While.fst"
-                                                                    (Prims.of_int (107))
+                                                                    (Prims.of_int (101))
                                                                     (Prims.of_int (11))
-                                                                    (Prims.of_int (112))
-                                                                    (Prims.of_int (74)))
+                                                                    (Prims.of_int (106))
+                                                                    (Prims.of_int (77)))
                                                                     (Obj.magic
                                                                     (FStar_Tactics_Effect.tac_bind
                                                                     (FStar_Range.mk_range
                                                                     "Pulse.Checker.While.fst"
-                                                                    (Prims.of_int (112))
+                                                                    (Prims.of_int (106))
                                                                     (Prims.of_int (33))
-                                                                    (Prims.of_int (112))
-                                                                    (Prims.of_int (73)))
+                                                                    (Prims.of_int (106))
+                                                                    (Prims.of_int (76)))
                                                                     (FStar_Range.mk_range
                                                                     "Pulse.Checker.While.fst"
-                                                                    (Prims.of_int (108))
+                                                                    (Prims.of_int (102))
                                                                     Prims.int_zero
-                                                                    (Prims.of_int (112))
-                                                                    (Prims.of_int (74)))
+                                                                    (Prims.of_int (106))
+                                                                    (Prims.of_int (77)))
                                                                     (Obj.magic
                                                                     (Pulse_Syntax_Printer.comp_to_string
                                                                     (Pulse_Typing.comp_while_cond
-                                                                    inv1)))
+                                                                    nm inv1)))
                                                                     (fun
-                                                                    uu___9 ->
+                                                                    uu___8 ->
                                                                     (fun
-                                                                    uu___9 ->
+                                                                    uu___8 ->
                                                                     Obj.magic
                                                                     (FStar_Tactics_Effect.tac_bind
                                                                     (FStar_Range.mk_range
                                                                     "Pulse.Checker.While.fst"
-                                                                    (Prims.of_int (108))
+                                                                    (Prims.of_int (102))
                                                                     Prims.int_zero
-                                                                    (Prims.of_int (112))
-                                                                    (Prims.of_int (74)))
+                                                                    (Prims.of_int (106))
+                                                                    (Prims.of_int (77)))
                                                                     (FStar_Range.mk_range
                                                                     "Pulse.Checker.While.fst"
-                                                                    (Prims.of_int (108))
+                                                                    (Prims.of_int (102))
                                                                     Prims.int_zero
-                                                                    (Prims.of_int (112))
-                                                                    (Prims.of_int (74)))
+                                                                    (Prims.of_int (106))
+                                                                    (Prims.of_int (77)))
                                                                     (Obj.magic
                                                                     (FStar_Tactics_Effect.tac_bind
                                                                     (FStar_Range.mk_range
                                                                     "Pulse.Checker.While.fst"
-                                                                    (Prims.of_int (111))
+                                                                    (Prims.of_int (105))
                                                                     (Prims.of_int (33))
-                                                                    (Prims.of_int (111))
+                                                                    (Prims.of_int (105))
                                                                     (Prims.of_int (61)))
                                                                     (FStar_Range.mk_range
                                                                     "FStar.Printf.fst"
@@ -913,39 +816,37 @@ let (check_while :
                                                                     (Pulse_Syntax_Printer.comp_to_string
                                                                     cond_comp))
                                                                     (fun
-                                                                    uu___10
-                                                                    ->
+                                                                    uu___9 ->
                                                                     FStar_Tactics_Effect.lift_div_tac
                                                                     (fun
-                                                                    uu___11
+                                                                    uu___10
                                                                     ->
                                                                     fun x1 ->
                                                                     Prims.strcat
                                                                     (Prims.strcat
                                                                     "Could not prove that the inferred type of the while condition matches the annotation\nInferred type = "
                                                                     (Prims.strcat
-                                                                    uu___10
+                                                                    uu___9
                                                                     "\nAnnotated type = "))
                                                                     (Prims.strcat
                                                                     x1 "\n")))))
                                                                     (fun
-                                                                    uu___10
-                                                                    ->
+                                                                    uu___9 ->
                                                                     FStar_Tactics_Effect.lift_div_tac
                                                                     (fun
-                                                                    uu___11
-                                                                    ->
                                                                     uu___10
-                                                                    uu___9))))
-                                                                    uu___9)))
+                                                                    ->
+                                                                    uu___9
+                                                                    uu___8))))
+                                                                    uu___8)))
                                                                     (fun
-                                                                    uu___9 ->
+                                                                    uu___8 ->
                                                                     FStar_Tactics_Derived.fail
-                                                                    uu___9)))
-                                                                    uu___7)))
-                                                                    uu___7)))
+                                                                    uu___8)))
                                                                     uu___6)))
                                                                     uu___6)))
+                                                                    uu___5)))
+                                                                    uu___5)))
                                                                     | 
                                                                     uu___4 ->
                                                                     Obj.repr
