pulse/lib/steel/pulse/Pulse.Checker.While.fst
@@ -14,15 +14,15 @@ module Framing = Pulse.Checker.Framing
 module Metatheory = Pulse.Typing.Metatheory
 module RU = Pulse.RuntimeUtils
 
-let while_cond_comp_typing (#g:env) (u:universe) (ty:term) (inv_body:term)
+let while_cond_comp_typing (#g:env) (u:universe) (x:ppname) (ty:term) (inv_body:term)
                            (inv_typing:tot_typing g (Tm_ExistsSL u (as_binder ty) inv_body) Tm_VProp)
-  : Metatheory.comp_typing_u g (comp_while_cond inv_body)
-  = Metatheory.admit_comp_typing g (comp_while_cond inv_body)
+  : Metatheory.comp_typing_u g (comp_while_cond x inv_body)
+  = Metatheory.admit_comp_typing g (comp_while_cond x inv_body)
 
-let while_body_comp_typing (#g:env) (u:universe) (ty:term) (inv_body:term)
+let while_body_comp_typing (#g:env) (u:universe) (x:ppname) (ty:term) (inv_body:term)
                            (inv_typing:tot_typing g (Tm_ExistsSL u (as_binder ty) inv_body) Tm_VProp)
-  : Metatheory.comp_typing_u g (comp_while_body inv_body)
-  = Metatheory.admit_comp_typing g (comp_while_body inv_body)
+  : Metatheory.comp_typing_u g (comp_while_body x inv_body)
+  = Metatheory.admit_comp_typing g (comp_while_body x inv_body)
 
 #push-options "--ifuel 2 --z3rlimit_factor 4"
 let check_while
@@ -37,13 +37,7 @@ let check_while
   let g = push_context "while loop" g in
   let Tm_While { invariant=inv; condition=cond; body; condition_var } = t.term in
   let (| ex_inv, inv_typing |) =
-    let inv =                 (Tm_ExistsSL u0 { binder_ppname=condition_var; binder_ty=tm_bool } inv) in
-
-    if RU.debug_at_level g "inference"
-    then (
-      T.print (Printf.sprintf "Annotated precondition of while loop: %s\n" (P.term_to_string inv))
-    ); 
-    check_vprop (push_context "invariant" g) inv
+    check_vprop (push_context "invariant" g) (Tm_ExistsSL u0 { binder_ppname=condition_var; binder_ty=tm_bool } inv)
   in
   if RU.debug_at_level g "inference"
   then (
@@ -53,12 +47,12 @@ let check_while
   | Inr f -> T.raise (Framing_failure f)
   | Inl framing_token ->
     match ex_inv with
-    | Tm_ExistsSL u {binder_ty=ty} inv ->
+    | Tm_ExistsSL u {binder_ppname=nm; binder_ty=ty} inv ->
       if not (eq_tm ty tm_bool) ||
         not (eq_univ u u0)
       then T.fail "While loop invariant is exists but its witness type is not bool"
       else begin
-        let while_cond_comp_typing = while_cond_comp_typing u ty inv inv_typing in
+        let while_cond_comp_typing = while_cond_comp_typing u nm ty inv inv_typing in
         let (| res_typing, cond_pre_typing, x, post_typing |) =
             Metatheory.(st_comp_typing_inversion (comp_typing_inversion while_cond_comp_typing))
         in
@@ -70,13 +64,13 @@ let check_while
           check' allow_inst
                  (push_context "while condition" g)
                  cond
-                 (comp_pre (comp_while_cond inv))
+                 (comp_pre (comp_while_cond nm inv))
                  cond_pre_typing
                  (Some while_cond_hint)
         in
-        if eq_comp cond_comp (comp_while_cond inv)
+        if eq_comp cond_comp (comp_while_cond nm inv)
         then begin
-          let while_body_comp_typing = while_body_comp_typing u ty inv inv_typing in
+          let while_body_comp_typing = while_body_comp_typing u nm ty inv inv_typing in
           let (| res_typing, body_pre_typing, x, post_typing |) = 
               Metatheory.(st_comp_typing_inversion (comp_typing_inversion while_body_comp_typing))
           in
@@ -88,11 +82,11 @@ let check_while
               check' allow_inst
                      (push_context "while body" g)
                      body
-                     (comp_pre (comp_while_body inv))
+                     (comp_pre (comp_while_body nm inv))
                      body_pre_typing
                      (Some while_post_hint)
           in
-          if eq_comp body_comp (comp_while_body inv)
+          if eq_comp body_comp (comp_while_body nm inv)
           then let d = T_While g inv cond body inv_typing cond_typing body_typing in
                let (| c, st_d |) = Framing.apply_frame pre_typing d framing_token in
                repack (| c, st_d |) post_hint
@@ -102,13 +96,13 @@ let check_while
                                      Inferred type = %s\n\
                                      Annotated type = %s\n"
                                      (P.comp_to_string body_comp)
-                                     (P.comp_to_string (comp_while_body inv)))
+                                     (P.comp_to_string (comp_while_body nm inv)))
       end
       else T.fail 
 (Printf.sprintf "Could not prove that the inferred type of the while condition matches the annotation\n\
                                  Inferred type = %s\n\
                                  Annotated type = %s\n"
                                  (P.comp_to_string cond_comp)
-                                 (P.comp_to_string (comp_while_cond inv)))
+                                 (P.comp_to_string (comp_while_cond nm inv)))
                 end
      | _ -> T.fail "Typechecked invariant is not an exists"
